nola/examples/rust_halt/box.v
@@ -105,42 +105,44 @@ Section ty_box.
   Qed.
 
   (** Read from [ty_box] *)
-  #[export] Instance read_ty_box `{!Ty (X:=X) T sz} {κ} :
-    Read κ (ty_box T) T (ty_box (ty_uninit sz)) id (λ _, ()) | 20.
+  #[export] Instance read_ty_box `{!Ty (X:=X) T sz} {κ d} :
+    Read κ (S d) (ty_box T) d T (ty_box (ty_uninit sz)) id (λ _, ()) | 20.
   Proof.
     split=> >. iIntros "$ $". rewrite ty_box_unseal /=.
     iDestruct 1 as (????[= ->]??) "(>$ & >† & T)". rewrite sem_cif_in /=.
     iMod (stored_acc with "T") as "T". iDestruct (ty_own_size with "T") as %?.
+    iDestruct (ty_own_depth (d':=d) with "T") as "T"; [lia|].
     iDestruct (ty_own_clair with "T") as "$"=>//.
     iMod (store_alloc (sty_pty (pty_uninit sz) _ _ _ _) with "[]")
       as "u"=>/=; [by iExists ()|].
-    iModIntro. iSplit=>//. iIntros "$ !>". iFrame "†". iExists _, _, _.
+    iModIntro. iSplit=>//. iIntros "$ !>". iFrame "†". iExists _, _.
     rewrite sem_cif_in /=. by iFrame.
   Qed.
   (** Reading a copyable object from [ty_box] *)
-  Lemma read_ty_box_copy `{!Ty (X:=X) T sz, !Copy T sz} {κ} :
-    Read κ (ty_box T) T (ty_box T) id id.
+  Lemma read_ty_box_copy `{!Ty (X:=X) T sz, !Copy T sz} {κ d} :
+    Read κ (S d) (ty_box T) d T (ty_box T) id id.
   Proof.
     split=> >. iIntros "$ $". rewrite ty_box_unseal /=.
     iDestruct 1 as (????[= ->]??) "(>$ & >† & T)". rewrite sem_cif_in /=.
     iMod (stored_acc with "T") as "#T". iDestruct (ty_own_size with "T") as %?.
-    iDestruct (ty_own_clair with "T") as "$"=>//.
+    iDestruct (ty_own_depth (d':=d) with "T") as "T'"; [lia|].
+    iDestruct (ty_own_clair with "T'") as "$"=>//.
     iMod (store_alloc with "T") as "{T}T". iModIntro. iSplit=>//.
-    iIntros "↦ !>". iFrame "↦ †". iExists _, _, _. rewrite sem_cif_in /=.
+    iIntros "↦ !>". iFrame "↦ †". iExists _, _. rewrite sem_cif_in /=.
     by iFrame.
   Qed.
 
   (** Write to [ty_box] *)
-  Lemma write_ty_box `{!Ty (X:=X) T sz, !Ty (X:=Y) U sz} {κ} :
-    Write κ (ty_box T) T U (ty_box U) id (λ _, id).
+  Lemma write_ty_box `{!Ty (X:=X) T sz, !Ty (X:=Y) U sz} {κ d d'} :
+    Write κ (S d) (ty_box T) d T d' U (S d') (ty_box U) id (λ _, id).
   Proof.
     split=> >. iIntros "$". rewrite ty_box_unseal /=.
     iDestruct 1 as (????[= ->]??) "(>$ & >† & T)". rewrite sem_cif_in /=.
     iMod (stored_acc with "T") as "T". iDestruct (ty_own_size with "T") as %->.
+    iDestruct (ty_own_depth (d':=d) with "T") as "T"; [lia|].
     iDestruct (ty_own_clair with "T") as "$"=>//. iModIntro. iSplit=>//.
-    iIntros (d' ??) "↦ U". iFrame "↦". iDestruct (ty_own_size with "U") as %->.
-    iMod (store_alloc with "U") as "U". iModIntro. iFrame "†".
-    iExists (S d'), _, _. rewrite sem_cif_in /=. iFrame "U". iPureIntro.
-    do 2 split=>//. lia.
+    iIntros (??) "↦ U". iFrame "↦". iDestruct (ty_own_size with "U") as %->.
+    iMod (store_alloc with "U") as "U". iModIntro. iFrame "†". iExists _, _.
+    rewrite sem_cif_in /=. iFrame "U". iPureIntro. do 2 split=>//. lia.
   Qed.
 End ty_box.
